src/Loops.v
@@ -24,46 +24,46 @@ Require Export Monads Globals.
 
 (** A structure to deal with infinite execution (which is not allowed in Coq). Inspired from JSCert. **)
 Record runs_type : Type := runs_type_intro {
-    runs_while_loop : forall A, state -> A -> (state -> A -> result bool) -> (state -> A -> result A) -> result A ;
-    runs_set_longjump : forall A, state -> context_type -> nat -> (state -> context_type -> result A) -> result A ;
-    runs_eval : state -> SEXP -> SEXP -> result SEXP ;
-    runs_getAttrib : state -> SEXP -> SEXP -> result SEXP ;
-    runs_setAttrib : state -> SEXP -> SEXP -> SEXP -> result SEXP ;
-    runs_R_cycle_detected : state -> SEXP -> SEXP -> result bool ;
-    runs_duplicate1 : state -> SEXP -> bool -> result SEXP ;
-    runs_stripAttrib : state -> SEXP -> SEXP -> result SEXP ;
-    runs_evalseq : state -> SEXP -> SEXP -> bool -> SEXP -> result SEXP ;
-    runs_R_isMissing : state -> SEXP -> SEXP -> result bool ;
-    runs_AnswerType : state -> SEXP -> bool -> bool -> BindData -> SEXP -> result BindData ;
-    runs_ListAnswer : state -> SEXP -> bool -> BindData -> SEXP -> result BindData ;
-    runs_StringAnswer : state -> SEXP -> BindData -> SEXP -> result BindData ;
-    runs_LogicalAnswer : state -> SEXP -> BindData -> SEXP -> result BindData ;
-    runs_IntegerAnswer : state -> SEXP -> BindData -> SEXP -> result BindData ;
-    runs_RealAnswer : state -> SEXP -> BindData -> SEXP -> result BindData ;
-    runs_ComplexAnswer : state -> SEXP -> BindData -> SEXP -> result BindData ;
-    runs_RawAnswer : state -> SEXP -> BindData -> SEXP -> result BindData ;
-    runs_substitute : state -> SEXP -> SEXP -> result SEXP ;
-    runs_substituteList : state -> SEXP -> SEXP -> result SEXP ;
+    runs_while_loop : forall A, A -> (A -> result bool) -> (A -> result A) -> result A ;
+    runs_set_longjump : forall A, context_type -> nat -> (context_type -> result A) -> result A ;
+    runs_eval : SEXP -> SEXP -> result SEXP ;
+    runs_getAttrib : SEXP -> SEXP -> result SEXP ;
+    runs_setAttrib : SEXP -> SEXP -> SEXP -> result SEXP ;
+    runs_R_cycle_detected : SEXP -> SEXP -> result bool ;
+    runs_duplicate1 : SEXP -> bool -> result SEXP ;
+    runs_stripAttrib : SEXP -> SEXP -> result SEXP ;
+    runs_evalseq : SEXP -> SEXP -> bool -> SEXP -> result SEXP ;
+    runs_R_isMissing : SEXP -> SEXP -> result bool ;
+    runs_AnswerType : SEXP -> bool -> bool -> BindData -> SEXP -> result BindData ;
+    runs_ListAnswer : SEXP -> bool -> BindData -> SEXP -> result BindData ;
+    runs_StringAnswer : SEXP -> BindData -> SEXP -> result BindData ;
+    runs_LogicalAnswer : SEXP -> BindData -> SEXP -> result BindData ;
+    runs_IntegerAnswer : SEXP -> BindData -> SEXP -> result BindData ;
+    runs_RealAnswer : SEXP -> BindData -> SEXP -> result BindData ;
+    runs_ComplexAnswer : SEXP -> BindData -> SEXP -> result BindData ;
+    runs_RawAnswer : SEXP -> BindData -> SEXP -> result BindData ;
+    runs_substitute : SEXP -> SEXP -> result SEXP ;
+    runs_substituteList : SEXP -> SEXP -> result SEXP ;
     runs_R_FunTab : option funtab
   }.
 
 (** The following function reads the [runs_R_FunTab] projection as a result. **)
-Definition get_R_FunTab runs S :=
+Definition get_R_FunTab runs :=
   add%stack "get_R_FunTab" in
   match runs_R_FunTab runs with
-  | None => result_bottom S
-  | Some t => result_success S t
+  | None => result_bottom
+  | Some t => result_success t
   end.
 
 (** An accessor for the [runs_R_FunTab] projection. **)
-Definition read_R_FunTab runs S n :=
+Definition read_R_FunTab runs n :=
   add%stack "read_R_FunTab" in
-  let%success t := get_R_FunTab runs S using S in
+  let%success t := get_R_FunTab runs in
   ifb n >= ArrayList.length t then
-    result_impossible S "Out of bounds."
+    result_impossible "Out of bounds."
   else
     let c := ArrayList.read t n in
-    result_success S c.
+    result_success c.
 
 
 (** * Frequent Patterns **)
@@ -74,223 +74,223 @@ Definition read_R_FunTab runs S n :=
 (** ** While **)
 
 (** A basic C-like loop **)
-Definition while_loop runs A S (a : A) expr stat : result A :=
-  if%success expr S a using S then
-    let%success a := stat S a using S in
-    runs_while_loop runs S a expr stat
+Definition while_loop runs A (a : A) expr stat : result A :=
+  if%success expr a then
+    let%success a := stat a in
+    runs_while_loop runs a expr stat
   else
-    result_success S a.
+    result_success a.
 
-Notation "'do%let' a ':=' e 'while' expr 'do' stat 'using' S ',' runs" :=
-  (while_loop runs S e (fun S a => expr) (fun S a => stat))
+Notation "'do%let' a ':=' e 'while' expr 'do' stat 'using' runs" :=
+  (while_loop runs e (fun a => expr) (fun a => stat))
   (at level 50, left associativity) : monad_scope.
 
-Notation "'do%let' 'while' expr 'do' stat 'using' S ',' runs" :=
+Notation "'do%let' 'while' expr 'do' stat 'using' runs" :=
   (do%let _ := tt
    while expr
    do stat
-   using S, runs)
+   using runs)
   (at level 50, left associativity) : monad_scope.
 
-Notation "'do%let' '(' a1 ',' a2 ')' ':=' a 'while' expr 'do' stat 'using' S ',' runs" :=
+Notation "'do%let' '(' a1 ',' a2 ')' ':=' a 'while' expr 'do' stat 'using' runs" :=
   (do%let x := a
    while let (a1, a2) := x in expr
    do let (a1, a2) := x in stat
-   using S, runs)
+   using runs)
   (at level 50, left associativity) : monad_scope.
 
-Notation "'do%let' '(' a1 ',' a2 ',' a3 ')' ':=' a 'while' expr 'do' stat 'using' S ',' runs" :=
+Notation "'do%let' '(' a1 ',' a2 ',' a3 ')' ':=' a 'while' expr 'do' stat 'using' runs" :=
   (do%let x := a
    while let '(a1, a2, a3) := x in expr
    do let '(a1, a2, a3) := x in stat
-   using S, runs)
+   using runs)
   (at level 50, left associativity) : monad_scope.
 
-Notation "'do%let' '(' a1 ',' a2 ',' a3 ',' a4 ')' ':=' a 'while' expr 'do' stat 'using' S ',' runs" :=
+Notation "'do%let' '(' a1 ',' a2 ',' a3 ',' a4 ')' ':=' a 'while' expr 'do' stat 'using' runs" :=
   (do%let x := a
    while let '(a1, a2, a3, a4) := x in expr
    do let '(a1, a2, a3, a4) := x in stat
-   using S, runs)
+   using runs)
   (at level 50, left associativity) : monad_scope.
 
-Notation "'do%let' '(' a1 ',' a2 ',' a3 ',' a4 ',' a5 ')' ':=' a 'while' expr 'do' stat 'using' S ',' runs" :=
+Notation "'do%let' '(' a1 ',' a2 ',' a3 ',' a4 ',' a5 ')' ':=' a 'while' expr 'do' stat 'using' runs" :=
   (do%let x := a
    while let '(a1, a2, a3, a4, a5) := x in expr
    do let '(a1, a2, a3, a4, a5) := x in stat
-   using S, runs)
+   using runs)
   (at level 50, left associativity) : monad_scope.
 
-Notation "'do%let' '(' a1 ',' a2 ',' a3 ',' a4 ',' a5 ',' a6 ')' ':=' a 'while' expr 'do' stat 'using' S ',' runs" :=
+Notation "'do%let' '(' a1 ',' a2 ',' a3 ',' a4 ',' a5 ',' a6 ')' ':=' a 'while' expr 'do' stat 'using' runs" :=
   (do%let x := a
    while let '(a1, a2, a3, a4, a5, a6) := x in expr
    do let '(a1, a2, a3, a4, a5, a6) := x in stat
-   using S, runs)
+   using runs)
   (at level 50, left associativity) : monad_scope.
 
-Notation "'do%let' a ':=' e 'whileb' expr 'do' stat 'using' S ',' runs" :=
+Notation "'do%let' a ':=' e 'whileb' expr 'do' stat 'using' runs" :=
   (do%let a := e
-   while result_success S (decide expr)
+   while result_success (decide expr)
    do stat
-   using S, runs)
+   using runs)
   (at level 50, left associativity) : monad_scope.
 
-Notation "'do%let' 'whileb' expr 'do' stat 'using' S ',' runs" :=
+Notation "'do%let' 'whileb' expr 'do' stat 'using' runs" :=
   (do%let
-   while result_success S (decide expr)
+   while result_success (decide expr)
    do stat
-   using S, runs)
+   using runs)
   (at level 50, left associativity) : monad_scope.
 
-Notation "'do%let' '(' a1 ',' a2 ')' ':=' a 'whileb' expr 'do' stat 'using' S ',' runs" :=
+Notation "'do%let' '(' a1 ',' a2 ')' ':=' a 'whileb' expr 'do' stat 'using' runs" :=
   (do%let (a1, a2) := a
-   while result_success S (decide expr)
+   while result_success (decide expr)
    do stat
-   using S, runs)
+   using runs)
   (at level 50, left associativity) : monad_scope.
 
-Notation "'do%let' '(' a1 ',' a2 ',' a3 ')' ':=' a 'whileb' expr 'do' stat 'using' S ',' runs" :=
+Notation "'do%let' '(' a1 ',' a2 ',' a3 ')' ':=' a 'whileb' expr 'do' stat 'using' runs" :=
   (do%let (a1, a2, a3) := a
-   while result_success S (decide expr)
+   while result_success (decide expr)
    do stat
-   using S, runs)
+   using runs)
   (at level 50, left associativity) : monad_scope.
 
-Notation "'do%let' '(' a1 ',' a2 ',' a3 ',' a4 ')' ':=' a 'whileb' expr 'do' stat 'using' S ',' runs" :=
+Notation "'do%let' '(' a1 ',' a2 ',' a3 ',' a4 ')' ':=' a 'whileb' expr 'do' stat 'using' runs" :=
   (do%let (a1, a2, a3, a4) := a
-   while result_success S (decide expr)
+   while result_success (decide expr)
    do stat
-   using S, runs)
+   using runs)
   (at level 50, left associativity) : monad_scope.
 
-Notation "'do%let' '(' a1 ',' a2 ',' a3 ',' a4 ',' a5 ')' ':=' a 'whileb' expr 'do' stat 'using' S ',' runs" :=
+Notation "'do%let' '(' a1 ',' a2 ',' a3 ',' a4 ',' a5 ')' ':=' a 'whileb' expr 'do' stat 'using' runs" :=
   (do%let (a1, a2, a3, a4, a5) := a
-   while result_success S (decide expr)
+   while result_success (decide expr)
    do stat
-   using S, runs)
+   using runs)
   (at level 50, left associativity) : monad_scope.
 
-Notation "'do%let' '(' a1 ',' a2 ',' a3 ',' a4 ',' a5 ',' a6 ')' ':=' a 'whileb' expr 'do' stat 'using' S ',' runs" :=
+Notation "'do%let' '(' a1 ',' a2 ',' a3 ',' a4 ',' a5 ',' a6 ')' ':=' a 'whileb' expr 'do' stat 'using' runs" :=
   (do%let (a1, a2, a3, a4, a5, a6) := a
-   while result_success S (decide expr)
+   while result_success (decide expr)
    do stat
-   using S, runs)
+   using runs)
   (at level 50, left associativity) : monad_scope.
 
-Notation "'do%success' 'while' expr 'do' stat 'using' S ',' runs 'in' cont" :=
+Notation "'do%success' 'while' expr 'do' stat 'using' runs 'in' cont" :=
   (run%success
      do%let while expr
      do stat
-     using S, runs using S in
+     using runs in
    cont)
   (at level 50, left associativity) : monad_scope.
 
-Notation "'do%success' a ':=' e 'while' expr 'do' stat 'using' S ',' runs 'in' cont" :=
+Notation "'do%success' a ':=' e 'while' expr 'do' stat 'using' runs 'in' cont" :=
   (let%success a :=
      do%let a := e
      while expr
      do stat
-     using S, runs using S in
+     using runs in
    cont)
   (at level 50, left associativity) : monad_scope.
 
-Notation "'do%success' '(' a1 ',' a2 ')' ':=' a 'while' expr 'do' stat 'using' S ',' runs 'in' cont" :=
+Notation "'do%success' '(' a1 ',' a2 ')' ':=' a 'while' expr 'do' stat 'using' runs 'in' cont" :=
   (let%success (a1, a2) :=
      do%let (a1, a2) := a
      while expr
      do stat
-     using S, runs using S in
+     using runs in
    cont)
   (at level 50, left associativity) : monad_scope.
 
-Notation "'do%success' '(' a1 ',' a2 ',' a3 ')' ':=' a 'while' expr 'do' stat 'using' S ',' runs 'in' cont" :=
+Notation "'do%success' '(' a1 ',' a2 ',' a3 ')' ':=' a 'while' expr 'do' stat 'using' runs 'in' cont" :=
   (let%success (a1, a2, a3) :=
      do%let (a1, a2, a3) := a
      while expr
      do stat
-     using S, runs using S in
+     using runs in
    cont)
   (at level 50, left associativity) : monad_scope.
 
-Notation "'do%success' '(' a1 ',' a2 ',' a3 ',' a4 ')' ':=' a 'while' expr 'do' stat 'using' S ',' runs 'in' cont" :=
+Notation "'do%success' '(' a1 ',' a2 ',' a3 ',' a4 ')' ':=' a 'while' expr 'do' stat 'using' runs 'in' cont" :=
   (let%success (a1, a2, a3, a4) :=
      do%let (a1, a2, a3, a4) := a
      while expr
      do stat
-     using S, runs using S in
+     using runs in
    cont)
   (at level 50, left associativity) : monad_scope.
 
-Notation "'do%success' '(' a1 ',' a2 ',' a3 ',' a4 ',' a5 ')' ':=' a 'while' expr 'do' stat 'using' S ',' runs 'in' cont" :=
+Notation "'do%success' '(' a1 ',' a2 ',' a3 ',' a4 ',' a5 ')' ':=' a 'while' expr 'do' stat 'using' runs 'in' cont" :=
   (let%success (a1, a2, a3, a4, a5) :=
      do%let (a1, a2, a3, a4, a5) := a
      while expr
      do stat
-     using S, runs using S in
+     using runs in
    cont)
   (at level 50, left associativity) : monad_scope.
 
-Notation "'do%success' '(' a1 ',' a2 ',' a3 ',' a4 ',' a5 ',' a6 ')' ':=' a 'while' expr 'do' stat 'using' S ',' runs 'in' cont" :=
+Notation "'do%success' '(' a1 ',' a2 ',' a3 ',' a4 ',' a5 ',' a6 ')' ':=' a 'while' expr 'do' stat 'using' runs 'in' cont" :=
   (let%success (a1, a2, a3, a4, a5, a6) :=
      do%let (a1, a2, a3, a4, a5, a6) := a
      while expr
      do stat
-     using S, runs using S in
+     using runs in
    cont)
   (at level 50, left associativity) : monad_scope.
 
-Notation "'do%success' 'whileb' expr 'do' stat 'using' S ',' runs 'in' cont" :=
+Notation "'do%success' 'whileb' expr 'do' stat 'using' runs 'in' cont" :=
   (do%success
-   while result_success S (decide expr)
+   while result_success (decide expr)
    do stat
-   using S, runs in
+   using runs in
    cont)
   (at level 50, left associativity) : monad_scope.
 
-Notation "'do%success' a ':=' e 'whileb' expr 'do' stat 'using' S ',' runs 'in' cont" :=
+Notation "'do%success' a ':=' e 'whileb' expr 'do' stat 'using' runs 'in' cont" :=
   (do%success a := e
-   while result_success S (decide expr)
+   while result_success (decide expr)
    do stat
-   using S, runs in
+   using runs in
    cont)
   (at level 50, left associativity) : monad_scope.
 
-Notation "'do%success' '(' a1 ',' a2 ')' ':=' a 'whileb' expr 'do' stat 'using' S ',' runs 'in' cont" :=
+Notation "'do%success' '(' a1 ',' a2 ')' ':=' a 'whileb' expr 'do' stat 'using' runs 'in' cont" :=
   (do%success (a1, a2) := a
-   while result_success S (decide expr)
+   while result_success (decide expr)
    do stat
-   using S, runs in
+   using runs in
    cont)
   (at level 50, left associativity) : monad_scope.
 
-Notation "'do%success' '(' a1 ',' a2 ',' a3 ')' ':=' a 'whileb' expr 'do' stat 'using' S ',' runs 'in' cont" :=
+Notation "'do%success' '(' a1 ',' a2 ',' a3 ')' ':=' a 'whileb' expr 'do' stat 'using' runs 'in' cont" :=
   (do%success (a1, a2, a3) := a
-   while result_success S (decide expr)
+   while result_success (decide expr)
    do stat
-   using S, runs in
+   using runs in
    cont)
   (at level 50, left associativity) : monad_scope.
 
-Notation "'do%success' '(' a1 ',' a2 ',' a3 ',' a4 ')' ':=' a 'whileb' expr 'do' stat 'using' S ',' runs 'in' cont" :=
+Notation "'do%success' '(' a1 ',' a2 ',' a3 ',' a4 ')' ':=' a 'whileb' expr 'do' stat 'using' runs 'in' cont" :=
   (do%success (a1, a2, a3, a4) := a
-   while result_success S (decide expr)
+   while result_success (decide expr)
    do stat
-   using S, runs in
+   using runs in
    cont)
   (at level 50, left associativity) : monad_scope.
 
-Notation "'do%success' '(' a1 ',' a2 ',' a3 ',' a4 ',' a5 ')' ':=' a 'whileb' expr 'do' stat 'using' S ',' runs 'in' cont" :=
+Notation "'do%success' '(' a1 ',' a2 ',' a3 ',' a4 ',' a5 ')' ':=' a 'whileb' expr 'do' stat 'using' runs 'in' cont" :=
   (do%success (a1, a2, a3, a4, a5) := a
-   while result_success S (decide expr)
+   while result_success (decide expr)
    do stat
-   using S, runs in
+   using runs in
    cont)
   (at level 50, left associativity) : monad_scope.
 
-Notation "'do%success' '(' a1 ',' a2 ',' a3 ',' a4 ',' a5 ',' a6 ')' ':=' a 'whileb' expr 'do' stat 'using' S ',' runs 'in' cont" :=
+Notation "'do%success' '(' a1 ',' a2 ',' a3 ',' a4 ',' a5 ',' a6 ')' ':=' a 'whileb' expr 'do' stat 'using' runs 'in' cont" :=
   (do%success (a1, a2, a3, a4, a5, a6) := a
-   while result_success S (decide expr)
+   while result_success (decide expr)
    do stat
-   using S, runs in
+   using runs in
    cont)
   (at level 50, left associativity) : monad_scope.
 
@@ -299,269 +299,269 @@ Notation "'do%success' '(' a1 ',' a2 ',' a3 ',' a4 ',' a5 ',' a6 ')' ':=' a 'whi
 (** Looping through a list is a frequent pattern in R source code.
   [fold_left_listSxp_gen] corresponds to the C code
   [for (i = l, v = a; i != R_NilValue; i = CDR (i)) v = iterate ( *i, v); v]. **)
-Definition fold_left_listSxp_gen runs (globals : Globals) A S (l : SEXP) (a : A)
-    (iterate : state -> A -> SEXP -> SExpRec -> ListSxp_struct -> result A) : result A :=
+Definition fold_left_listSxp_gen runs (globals : Globals) A (l : SEXP) (a : A)
+    (iterate : A -> SEXP -> SExpRec -> ListSxp_struct -> result A) : result A :=
   do%success (l, a) := (l, a)
   whileb l <> global_mapping globals R_NilValue
   do
-    read%list l_, l_list := l using S in
-    let%success a := iterate S a l l_ l_list using S in
-    result_success S (list_cdrval l_list, a)
-  using S, runs in
-  result_success S a.
+    read%list l_, l_list := l in
+    let%success a := iterate a l l_ l_list in
+    result_success (list_cdrval l_list, a)
+  using runs in
+  result_success a.
 
-Notation "'fold%let' a ':=' e 'along' le 'as' l ',' l_ ',' l_list 'do' iterate 'using' S ',' runs ',' globals" :=
-  (fold_left_listSxp_gen runs globals S le e (fun S a l l_ l_list => iterate))
+Notation "'fold%let' a ':=' e 'along' le 'as' l ',' l_ ',' l_list 'do' iterate 'using' runs ',' globals" :=
+  (fold_left_listSxp_gen runs globals le e (fun a l l_ l_list => iterate))
   (at level 50, left associativity) : monad_scope.
 
-Notation "'fold%let' 'along' le 'as' l ',' l_ ',' l_list 'do' iterate 'using' S ',' runs ',' globals" :=
+Notation "'fold%let' 'along' le 'as' l ',' l_ ',' l_list 'do' iterate 'using' runs ',' globals" :=
   (fold%let _ := tt
    along le
    as l, l_, l_list
    do iterate
-   using S, runs, globals)
+   using runs, globals)
   (at level 50, left associativity) : monad_scope.
 
-Notation "'fold%let' '(' a1 ',' a2 ')' ':=' e 'along' le 'as' l ',' l_ ',' l_list 'do' iterate 'using' S ',' runs ',' globals" :=
+Notation "'fold%let' '(' a1 ',' a2 ')' ':=' e 'along' le 'as' l ',' l_ ',' l_list 'do' iterate 'using' runs ',' globals" :=
   (fold%let x := e
    along le
    as l, l_, l_list
    do let (a1, a2) := x in iterate
-   using S, runs, globals)
+   using runs, globals)
   (at level 50, left associativity) : monad_scope.
 
-Notation "'fold%let' '(' a1 ',' a2 ',' a3 ')' ':=' e 'along' le 'as' l ',' l_ ',' l_list 'do' iterate 'using' S ',' runs ',' globals" :=
+Notation "'fold%let' '(' a1 ',' a2 ',' a3 ')' ':=' e 'along' le 'as' l ',' l_ ',' l_list 'do' iterate 'using' runs ',' globals" :=
   (fold%let x := e
    along le
    as l, l_, l_list
    do let '(a1, a2, a3) := x in iterate
-   using S, runs, globals)
+   using runs, globals)
   (at level 50, left associativity) : monad_scope.
 
-Notation "'fold%let' '(' a1 ',' a2 ',' a3 ',' a4 ')' ':=' e 'along' le 'as' l ',' l_ ',' l_list 'do' iterate 'using' S ',' runs ',' globals" :=
+Notation "'fold%let' '(' a1 ',' a2 ',' a3 ',' a4 ')' ':=' e 'along' le 'as' l ',' l_ ',' l_list 'do' iterate 'using' runs ',' globals" :=
   (fold%let x := e
    along le
    as l, l_, l_list
    do let '(a1, a2, a3, a4) := x in iterate
-   using S, runs, globals)
+   using runs, globals)
   (at level 50, left associativity) : monad_scope.
 
-Notation "'fold%let' '(' a1 ',' a2 ',' a3 ',' a4 ',' a5 ')' ':=' e 'along' le 'as' l ',' l_ ',' l_list 'do' iterate 'using' S ',' runs ',' globals" :=
+Notation "'fold%let' '(' a1 ',' a2 ',' a3 ',' a4 ',' a5 ')' ':=' e 'along' le 'as' l ',' l_ ',' l_list 'do' iterate 'using' runs ',' globals" :=
   (fold%let x := e
    along le
    as l, l_, l_list
    do let '(a1, a2, a3, a4, a5) := x in iterate
-   using S, runs, globals)
+   using runs, globals)
   (at level 50, left associativity) : monad_scope.
 
-Notation "'fold%let' '(' a1 ',' a2 ',' a3 ',' a4 ',' a5 ',' a6 ')' ':=' e 'along' le 'as' l ',' l_ ',' l_list 'do' iterate 'using' S ',' runs ',' globals" :=
+Notation "'fold%let' '(' a1 ',' a2 ',' a3 ',' a4 ',' a5 ',' a6 ')' ':=' e 'along' le 'as' l ',' l_ ',' l_list 'do' iterate 'using' runs ',' globals" :=
   (fold%let x := e
    along le
    as l, l_, l_list
    do let '(a1, a2, a3, a4, a5, a6) := x in iterate
-   using S, runs, globals)
+   using runs, globals)
   (at level 50, left associativity) : monad_scope.
 
-Notation "'fold%success' 'along' le 'as' l ',' l_ ',' l_list 'do' iterate 'using' S ',' runs ',' globals 'in' cont" :=
+Notation "'fold%success' 'along' le 'as' l ',' l_ ',' l_list 'do' iterate 'using' runs ',' globals 'in' cont" :=
   (run%success
      fold%let
      along le
      as l, l_, l_list
      do iterate
-     using S, runs, globals using S in
+     using runs, globals in
    cont)
     (at level 50, left associativity) : monad_scope.
 
-Notation "'fold%success' a ':=' e 'along' le 'as' l ',' l_ ',' l_list 'do' iterate 'using' S ',' runs ',' globals 'in' cont" :=
+Notation "'fold%success' a ':=' e 'along' le 'as' l ',' l_ ',' l_list 'do' iterate 'using' runs ',' globals 'in' cont" :=
   (let%success a :=
      fold%let a := e
      along le
      as l, l_, l_list
      do iterate
-     using S, runs, globals using S in
+     using runs, globals in
    cont)
   (at level 50, left associativity) : monad_scope.
 
-Notation "'fold%success' '(' a1 ',' a2 ')' ':=' e 'along' le 'as' l ',' l_ ',' l_list 'do' iterate 'using' S ',' runs ',' globals 'in' cont" :=
+Notation "'fold%success' '(' a1 ',' a2 ')' ':=' e 'along' le 'as' l ',' l_ ',' l_list 'do' iterate 'using' runs ',' globals 'in' cont" :=
   (let%success (a1, a2) :=
      fold%let (a1, a2) := e
      along le
      as l, l_, l_list
      do iterate
-     using S, runs, globals using S in
+     using runs, globals in
    cont)
   (at level 50, left associativity) : monad_scope.
 
-Notation "'fold%success' '(' a1 ',' a2 ',' a3 ')' ':=' e 'along' le 'as' l ',' l_ ',' l_list 'do' iterate 'using' S ',' runs ',' globals 'in' cont" :=
+Notation "'fold%success' '(' a1 ',' a2 ',' a3 ')' ':=' e 'along' le 'as' l ',' l_ ',' l_list 'do' iterate 'using' runs ',' globals 'in' cont" :=
   (let%success (a1, a2, a3) :=
      fold%let (a1, a2, a3) := e
      along le
      as l, l_, l_list
      do iterate
-     using S, runs, globals using S in
+     using runs, globals in
    cont)
   (at level 50, left associativity) : monad_scope.
 
-Notation "'fold%success' '(' a1 ',' a2 ',' a3 ',' a4 ')' ':=' e 'along' le 'as' l ',' l_ ',' l_list 'do' iterate 'using' S ',' runs ',' globals 'in' cont" :=
+Notation "'fold%success' '(' a1 ',' a2 ',' a3 ',' a4 ')' ':=' e 'along' le 'as' l ',' l_ ',' l_list 'do' iterate 'using' runs ',' globals 'in' cont" :=
   (let%success (a1, a2, a3, a4) :=
      fold%let (a1, a2, a3, a4) := e
      along le
      as l, l_, l_list
      do iterate
-     using S, runs, globals using S in
+     using runs, globals in
    cont)
   (at level 50, left associativity) : monad_scope.
 
-Notation "'fold%success' '(' a1 ',' a2 ',' a3 ',' a4 ',' a5 ')' ':=' e 'along' le 'as' l ',' l_ ',' l_list 'do' iterate 'using' S ',' runs ',' globals 'in' cont" :=
+Notation "'fold%success' '(' a1 ',' a2 ',' a3 ',' a4 ',' a5 ')' ':=' e 'along' le 'as' l ',' l_ ',' l_list 'do' iterate 'using' runs ',' globals 'in' cont" :=
   (let%success (a1, a2, a3, a4, a5) :=
      fold%let (a1, a2, a3, a4, a5) := e
      along le
      as l, l_, l_list
      do iterate
-     using S, runs, globals using S in
+     using runs, globals in
    cont)
   (at level 50, left associativity) : monad_scope.
 
-Notation "'fold%success' '(' a1 ',' a2 ',' a3 ',' a4 ',' a5 ',' a6 ')' ':=' e 'along' le 'as' l ',' l_ ',' l_list 'do' iterate 'using' S ',' runs ',' globals 'in' cont" :=
+Notation "'fold%success' '(' a1 ',' a2 ',' a3 ',' a4 ',' a5 ',' a6 ')' ':=' e 'along' le 'as' l ',' l_ ',' l_list 'do' iterate 'using' runs ',' globals 'in' cont" :=
   (let%success (a1, a2, a3, a4, a5, a6) :=
      fold%let (a1, a2, a3, a4, a5, a6) := e
      along le
      as l, l_, l_list
      do iterate
-     using S, runs, globals using S in
+     using runs, globals in
    cont)
   (at level 50, left associativity) : monad_scope.
 
 
 (** [fold_left_listSxp] corresponds to the C code
   [for (i = l, v = a; i != R_NilValue; i = CDR (i)) v = iterate (CAR (i), TAG (i), v); v]. **)
-Definition fold_left_listSxp runs globals A S (l : SEXP) (a : A)
-    (iterate : state -> A -> SEXP -> SEXP -> result A) : result A :=
+Definition fold_left_listSxp runs globals A (l : SEXP) (a : A)
+    (iterate : A -> SEXP -> SEXP -> result A) : result A :=
   fold%let a := a
   along l
   as _, _, l_list
-  do iterate S a (list_carval l_list) (list_tagval l_list)
-  using S, runs, globals.
+  do iterate a (list_carval l_list) (list_tagval l_list)
+  using runs, globals.
 
-Notation "'fold%let' a ':=' e 'along' le 'as' l_car ',' l_tag 'do' iterate 'using' S ',' runs ',' globals" :=
-  (fold_left_listSxp runs globals S le e (fun S a l_car l_tag => iterate))
+Notation "'fold%let' a ':=' e 'along' le 'as' l_car ',' l_tag 'do' iterate 'using' runs ',' globals" :=
+  (fold_left_listSxp runs globals le e (fun a l_car l_tag => iterate))
   (at level 50, left associativity) : monad_scope.
 
-Notation "'fold%let' 'along' le 'as' l_car ',' l_tag 'do' iterate 'using' S ',' runs ',' globals" :=
+Notation "'fold%let' 'along' le 'as' l_car ',' l_tag 'do' iterate 'using' runs ',' globals" :=
   (fold%let _ := tt
    along le
    as l_car, l_tag
    do iterate
-   using S, runs, globals)
+   using runs, globals)
   (at level 50, left associativity) : monad_scope.
 
-Notation "'fold%let' '(' a1 ',' a2 ')' ':=' e 'along' le 'as' l_car ',' l_tag 'do' iterate 'using' S ',' runs ',' globals" :=
+Notation "'fold%let' '(' a1 ',' a2 ')' ':=' e 'along' le 'as' l_car ',' l_tag 'do' iterate 'using' runs ',' globals" :=
   (fold%let x := e
    along le
    as l_car, l_tag
    do let (a1, a2) := x in iterate
-   using S, runs, globals)
+   using runs, globals)
   (at level 50, left associativity) : monad_scope.
 
-Notation "'fold%let' '(' a1 ',' a2 ',' a3 ')' ':=' e 'along' le 'as' l_car ',' l_tag 'do' iterate 'using' S ',' runs ',' globals" :=
+Notation "'fold%let' '(' a1 ',' a2 ',' a3 ')' ':=' e 'along' le 'as' l_car ',' l_tag 'do' iterate 'using' runs ',' globals" :=
   (fold%let x := e
    along le
    as l_car, l_tag
    do let '(a1, a2, a3) := x in iterate
-   using S, runs, globals)
+   using runs, globals)
   (at level 50, left associativity) : monad_scope.
 
-Notation "'fold%let' '(' a1 ',' a2 ',' a3 ',' a4 ')' ':=' e 'along' le 'as' l_car ',' l_tag 'do' iterate 'using' S ',' runs ',' globals" :=
+Notation "'fold%let' '(' a1 ',' a2 ',' a3 ',' a4 ')' ':=' e 'along' le 'as' l_car ',' l_tag 'do' iterate 'using' runs ',' globals" :=
   (fold%let x := e
    along le
    as l_car, l_tag
    do let '(a1, a2, a3, a4) := x in iterate
-   using S, runs, globals)
+   using runs, globals)
   (at level 50, left associativity) : monad_scope.
 
-Notation "'fold%let' '(' a1 ',' a2 ',' a3 ',' a4 ',' a5 ')' ':=' e 'along' le 'as' l_car ',' l_tag 'do' iterate 'using' S ',' runs ',' globals" :=
+Notation "'fold%let' '(' a1 ',' a2 ',' a3 ',' a4 ',' a5 ')' ':=' e 'along' le 'as' l_car ',' l_tag 'do' iterate 'using' runs ',' globals" :=
   (fold%let x := e
    along le
    as l_car, l_tag
    do let '(a1, a2, a3, a4, a5) := x in iterate
-   using S, runs, globals)
+   using runs, globals)
   (at level 50, left associativity) : monad_scope.
 
-Notation "'fold%let' '(' a1 ',' a2 ',' a3 ',' a4 ',' a5 ',' a6 ')' ':=' e 'along' le 'as' l_car ',' l_tag 'do' iterate 'using' S ',' runs ',' globals" :=
+Notation "'fold%let' '(' a1 ',' a2 ',' a3 ',' a4 ',' a5 ',' a6 ')' ':=' e 'along' le 'as' l_car ',' l_tag 'do' iterate 'using' runs ',' globals" :=
   (fold%let x := e
    along le
    as l_car, l_tag
    do let '(a1, a2, a3, a4, a5, a6) := x in iterate
-   using S, runs, globals)
+   using runs, globals)
   (at level 50, left associativity) : monad_scope.
 
-Notation "'fold%success' 'along' le 'as' l_car ',' l_tag 'do' iterate 'using' S ',' runs ',' globals 'in' cont" :=
+Notation "'fold%success' 'along' le 'as' l_car ',' l_tag 'do' iterate 'using' runs ',' globals 'in' cont" :=
   (run%success
      fold%let _ := tt
      along le
      as l_car, l_tag
      do iterate
-     using S, runs, globals using S in
+     using runs, globals in
    cont)
   (at level 50, left associativity) : monad_scope.
 
-Notation "'fold%success' a ':=' e 'along' le 'as' l_car ',' l_tag 'do' iterate 'using' S ',' runs ',' globals 'in' cont" :=
+Notation "'fold%success' a ':=' e 'along' le 'as' l_car ',' l_tag 'do' iterate 'using' runs ',' globals 'in' cont" :=
   (let%success a :=
      fold%let a := e
      along le
      as l_car, l_tag
      do iterate
-     using S, runs, globals using S in
+     using runs, globals in
    cont)
   (at level 50, left associativity) : monad_scope.
 
-Notation "'fold%success' '(' a1 ',' a2 ')' ':=' e 'along' le 'as' l_car ',' l_tag 'do' iterate 'using' S ',' runs ',' globals 'in' cont" :=
+Notation "'fold%success' '(' a1 ',' a2 ')' ':=' e 'along' le 'as' l_car ',' l_tag 'do' iterate 'using' runs ',' globals 'in' cont" :=
   (let%success (a1, a2) :=
      fold%let (a1, a2) := e
      along le
      as l_car, l_tag
      do iterate
-     using S, runs, globals using S in
+     using runs, globals in
    cont)
   (at level 50, left associativity) : monad_scope.
 
-Notation "'fold%success' '(' a1 ',' a2 ',' a3 ')' ':=' e 'along' le 'as' l_car ',' l_tag 'do' iterate 'using' S ',' runs ',' globals 'in' cont" :=
+Notation "'fold%success' '(' a1 ',' a2 ',' a3 ')' ':=' e 'along' le 'as' l_car ',' l_tag 'do' iterate 'using' runs ',' globals 'in' cont" :=
   (let%success (a1, a2, a3) :=
      fold%let (a1, a2, a3) := e
      along le
      as l_car, l_tag
      do iterate
-     using S, runs, globals using S in
+     using runs, globals in
    cont)
   (at level 50, left associativity) : monad_scope.
 
-Notation "'fold%success' '(' a1 ',' a2 ',' a3 ',' a4 ')' ':=' e 'along' le 'as' l_car ',' l_tag 'do' iterate 'using' S ',' runs ',' globals 'in' cont" :=
+Notation "'fold%success' '(' a1 ',' a2 ',' a3 ',' a4 ')' ':=' e 'along' le 'as' l_car ',' l_tag 'do' iterate 'using' runs ',' globals 'in' cont" :=
   (let%success (a1, a2, a3, a4) :=
      fold%let (a1, a2, a3, a4) := e
      along le
      as l_car, l_tag
      do iterate
-     using S, runs, globals using S in
+     using runs, globals in
    cont)
   (at level 50, left associativity) : monad_scope.
 
-Notation "'fold%success' '(' a1 ',' a2 ',' a3 ',' a4 ',' a5 ')' ':=' e 'along' le 'as' l_car ',' l_tag 'do' iterate 'using' S ',' runs ',' globals 'in' cont" :=
+Notation "'fold%success' '(' a1 ',' a2 ',' a3 ',' a4 ',' a5 ')' ':=' e 'along' le 'as' l_car ',' l_tag 'do' iterate 'using' runs ',' globals 'in' cont" :=
   (let%success (a1, a2, a3, a4, a5) :=
      fold%let (a1, a2, a3, a4, a5) := e
      along le
      as l_car, l_tag
      do iterate
-     using S, runs, globals using S in
+     using runs, globals in
    cont)
   (at level 50, left associativity) : monad_scope.
 
-Notation "'fold%success' '(' a1 ',' a2 ',' a3 ',' a4 ',' a5 ',' a6 ')' ':=' e 'along' le 'as' l_car ',' l_tag 'do' iterate 'using' S ',' runs ',' globals 'in' cont" :=
+Notation "'fold%success' '(' a1 ',' a2 ',' a3 ',' a4 ',' a5 ',' a6 ')' ':=' e 'along' le 'as' l_car ',' l_tag 'do' iterate 'using' runs ',' globals 'in' cont" :=
   (let%success (a1, a2, a3, a4, a5, a6) :=
      fold%let (a1, a2, a3, a4, a5, a6) := e
      along le
      as l_car, l_tag
      do iterate
-     using S, runs, globals using S in
+     using runs, globals in
    cont)
   (at level 50, left associativity) : monad_scope.
 
@@ -582,53 +582,53 @@ Inductive normal_return A B :=
 Arguments normal_result {A B}.
 Arguments return_result {A B}.
 
-Definition result_rsuccess {A B} S r : result (normal_return A B) :=
-  result_success S (normal_result r).
+Definition result_rsuccess {A B} r : result (normal_return A B) :=
+  result_success (normal_result r).
 
-Definition result_rskip {B} S : result (normal_return _ B) :=
-  result_rsuccess S tt.
+Definition result_rskip {B} : result (normal_return _ B) :=
+  result_rsuccess tt.
 
-Definition result_rreturn {A B} S r : result (normal_return A B) :=
-  result_success S (return_result r).
+Definition result_rreturn {A B} r : result (normal_return A B) :=
+  result_success (return_result r).
 
 Definition match_rresult {A B C} (r : result (normal_return A B)) cont
     : result (normal_return C B) :=
-  let%success res := r using S in
+  let%success res := r in
   match res with
-  | normal_result r => cont S r
-  | return_result r => result_rreturn S r
+  | normal_result r => cont r
+  | return_result r => result_rreturn r
   end.
 
-Notation "'let%return' a ':=' e 'using' S 'in' cont" :=
-  (match_rresult e (fun S a => cont))
+Notation "'let%return' a ':=' e 'in' cont" :=
+  (match_rresult e (fun a => cont))
   (at level 50, left associativity) : monad_scope.
 
-Notation "'run%return' c 'using' S 'in' cont" :=
-  (let%return _ := c using S in cont)
+Notation "'run%return' c 'in' cont" :=
+  (let%return _ := c in cont)
   (at level 50, left associativity) : monad_scope.
 
-Notation "'let%return' '(' a1 ',' a2 ')' ':=' e 'using' S 'in' cont" :=
-  (let%return a := e using S in
+Notation "'let%return' '(' a1 ',' a2 ')' ':=' e 'in' cont" :=
+  (let%return a := e in
    let (a1, a2) := a in cont)
   (at level 50, left associativity) : monad_scope.
 
-Notation "'let%return' '(' a1 ',' a2 ',' a3 ')' ':=' e 'using' S 'in' cont" :=
-  (let%return a := e using S in
+Notation "'let%return' '(' a1 ',' a2 ',' a3 ')' ':=' e 'in' cont" :=
+  (let%return a := e in
    let '(a1, a2, a3) := a in cont)
   (at level 50, left associativity) : monad_scope.
 
-Notation "'let%return' '(' a1 ',' a2 ',' a3 ',' a4 ')' ':=' e 'using' S 'in' cont" :=
-  (let%return a := e using S in
+Notation "'let%return' '(' a1 ',' a2 ',' a3 ',' a4 ')' ':=' e 'in' cont" :=
+  (let%return a := e in
    let '(a1, a2, a3, a4) := a in cont)
   (at level 50, left associativity) : monad_scope.
 
-Notation "'let%return' '(' a1 ',' a2 ',' a3 ',' a4 ',' a5 ')' ':=' e 'using' S 'in' cont" :=
-  (let%return a := e using S in
+Notation "'let%return' '(' a1 ',' a2 ',' a3 ',' a4 ',' a5 ')' ':=' e 'in' cont" :=
+  (let%return a := e in
    let '(a1, a2, a3, a4, a5) := a in cont)
   (at level 50, left associativity) : monad_scope.
 
-Notation "'let%return' '(' a1 ',' a2 ',' a3 ',' a4 ',' a5 ',' a6 ')' ':=' e 'using' S 'in' cont" :=
-  (let%return a := e using S in
+Notation "'let%return' '(' a1 ',' a2 ',' a3 ',' a4 ',' a5 ',' a6 ')' ':=' e 'in' cont" :=
+  (let%return a := e in
    let '(a1, a2, a3, a4, a5, a6) := a in cont)
   (at level 50, left associativity) : monad_scope.
 
@@ -636,377 +636,377 @@ Notation "'let%return' '(' a1 ',' a2 ',' a3 ',' a4 ',' a5 ',' a6 ')' ':=' e 'usi
 
 (** Exiting the return-monad. **)
 Definition exit_rresult {A B} (r : result (normal_return A B)) cont :=
-  let%success res := r using S in
+  let%success res := r in
   match res with
-  | normal_result r => cont S r
-  | return_result r => result_success S r
+  | normal_result r => cont r
+  | return_result r => result_success r
   end.
 
-Notation "'let%exit' a ':=' e 'using' S 'in' cont" :=
-  (exit_rresult e (fun S a => cont))
+Notation "'let%exit' a ':=' e 'in' cont" :=
+  (exit_rresult e (fun a => cont))
   (at level 50, left associativity) : monad_scope.
 
-Notation "'run%exit' c 'using' S 'in' cont" :=
-  (let%exit _ := c using S in cont)
+Notation "'run%exit' c 'in' cont" :=
+  (let%exit _ := c in cont)
   (at level 50, left associativity) : monad_scope.
 
-Notation "'let%exit' '(' a1 ',' a2 ')' ':=' e 'using' S 'in' cont" :=
-  (let%exit a := e using S in
+Notation "'let%exit' '(' a1 ',' a2 ')' ':=' e 'in' cont" :=
+  (let%exit a := e in
    let (a1, a2) := a in cont)
   (at level 50, left associativity) : monad_scope.
 
-Notation "'let%exit' '(' a1 ',' a2 ',' a3 ')' ':=' e 'using' S 'in' cont" :=
-  (let%exit a := e using S in
+Notation "'let%exit' '(' a1 ',' a2 ',' a3 ')' ':=' e 'in' cont" :=
+  (let%exit a := e in
    let '(a1, a2, a3) := a in cont)
   (at level 50, left associativity) : monad_scope.
 
-Notation "'let%exit' '(' a1 ',' a2 ',' a3 ',' a4 ')' ':=' e 'using' S 'in' cont" :=
-  (let%exit a := e using S in
+Notation "'let%exit' '(' a1 ',' a2 ',' a3 ',' a4 ')' ':=' e 'in' cont" :=
+  (let%exit a := e in
    let '(a1, a2, a3, a4) := a in cont)
   (at level 50, left associativity) : monad_scope.
 
-Notation "'let%exit' '(' a1 ',' a2 ',' a3 ',' a4 ',' a5 ')' ':=' e 'using' S 'in' cont" :=
-  (let%exit a := e using S in
+Notation "'let%exit' '(' a1 ',' a2 ',' a3 ',' a4 ',' a5 ')' ':=' e 'in' cont" :=
+  (let%exit a := e in
    let '(a1, a2, a3, a4, a5) := a in cont)
   (at level 50, left associativity) : monad_scope.
 
-Notation "'let%exit' '(' a1 ',' a2 ',' a3 ',' a4 ',' a5 ',' a6 ')' ':=' e 'using' S 'in' cont" :=
-  (let%exit a := e using S in
+Notation "'let%exit' '(' a1 ',' a2 ',' a3 ',' a4 ',' a5 ',' a6 ')' ':=' e 'in' cont" :=
+  (let%exit a := e in
    let '(a1, a2, a3, a4, a5, a6) := a in cont)
   (at level 50, left associativity) : monad_scope.
 
 
-Definition continue_and_condition {A B} S (r : normal_return A B) cond :=
+Definition continue_and_condition {A B} (r : normal_return A B) cond :=
   match r with
-  | normal_result r => cond S r
-  | return_result r => result_success S false
+  | normal_result r => cond r
+  | return_result r => result_success false
   end.
 
-Definition get_success {A B} S (r : normal_return A B) cont
+Definition get_success {A B} (r : normal_return A B) cont
     : result (normal_return A B) :=
   match r with
-  | normal_result r => cont S r
-  | return_result r => result_rreturn S r
+  | normal_result r => cont r
+  | return_result r => result_rreturn r
   end.
 
 
-Notation "'do%return' a ':=' e 'while' expr 'do' stat 'using' S ',' runs 'in' cont" :=
+Notation "'do%return' a ':=' e 'while' expr 'do' stat 'using' runs 'in' cont" :=
   (let%exit a :=
      do%let a := normal_result e
-     while continue_and_condition S a (fun S a => expr)
-     do get_success S a (fun S a => stat)
-     using S, runs
-   using S in cont)
+     while continue_and_condition a (fun a => expr)
+     do get_success a (fun a => stat)
+     using runs
+    in cont)
   (at level 50, left associativity) : monad_scope.
 
-Notation "'do%return' 'while' expr 'do' stat 'using' S ',' runs 'in' cont" :=
+Notation "'do%return' 'while' expr 'do' stat 'using' runs 'in' cont" :=
   (do%return _ := tt
    while expr
    do stat
-   using S, runs
+   using runs
    in cont)
   (at level 50, left associativity) : monad_scope.
 
-Notation "'do%return' '(' a1 ',' a2 ')' ':=' e 'while' expr 'do' stat 'using' S ',' runs 'in' cont" :=
+Notation "'do%return' '(' a1 ',' a2 ')' ':=' e 'while' expr 'do' stat 'using' runs 'in' cont" :=
   (do%return a := e
    while let (a1, a2) := a in expr
    do let (a1, a2) := a in stat
-   using S, runs
+   using runs
    in let (a1, a2) := a in cont)
   (at level 50, left associativity) : monad_scope.
 
-Notation "'do%return' '(' a1 ',' a2 ',' a3 ')' ':=' e 'while' expr 'do' stat 'using' S ',' runs 'in' cont" :=
+Notation "'do%return' '(' a1 ',' a2 ',' a3 ')' ':=' e 'while' expr 'do' stat 'using' runs 'in' cont" :=
   (do%return a := e
    while let (a1, a2, a3) := a in expr
    do let (a1, a2, a3) := a in stat
-   using S, runs
+   using runs
    in let (a1, a2, a3) := a in cont)
   (at level 50, left associativity) : monad_scope.
 
-Notation "'do%return' '(' a1 ',' a2 ',' a3 ',' a4 ')' ':=' e 'while' expr 'do' stat 'using' S ',' runs 'in' cont" :=
+Notation "'do%return' '(' a1 ',' a2 ',' a3 ',' a4 ')' ':=' e 'while' expr 'do' stat 'using' runs 'in' cont" :=
   (do%return a := e
    while let (a1, a2, a3, a4) := a in expr
    do let (a1, a2, a3, a4) := a in stat
-   using S, runs
+   using runs
    in let (a1, a2, a3, a4) := a in cont)
   (at level 50, left associativity) : monad_scope.
 
-Notation "'do%return' '(' a1 ',' a2 ',' a3 ',' a4 ',' a5 ')' ':=' e 'while' expr 'do' stat 'using' S ',' runs 'in' cont" :=
+Notation "'do%return' '(' a1 ',' a2 ',' a3 ',' a4 ',' a5 ')' ':=' e 'while' expr 'do' stat 'using' runs 'in' cont" :=
   (do%return a := e
    while let (a1, a2, a3, a4, a5) := a in expr
    do let (a1, a2, a3, a4, a5) := a in stat
-   using S, runs
+   using runs
    in let (a1, a2, a3, a4, a5) := a in cont)
   (at level 50, left associativity) : monad_scope.
 
-Notation "'do%return' '(' a1 ',' a2 ',' a3 ',' a4 ',' a5 ',' a6 ')' ':=' e 'while' expr 'do' stat 'using' S ',' runs 'in' cont" :=
+Notation "'do%return' '(' a1 ',' a2 ',' a3 ',' a4 ',' a5 ',' a6 ')' ':=' e 'while' expr 'do' stat 'using' runs 'in' cont" :=
   (do%return a := e
    while let (a1, a2, a3, a4, a5, a6) := a in expr
    do let (a1, a2, a3, a4, a5, a6) := a in stat
-   using S, runs
+   using runs
    in let (a1, a2, a3, a4, a5, a6) := a in cont)
   (at level 50, left associativity) : monad_scope.
 
-Notation "'do%return' a ':=' e 'whileb' expr 'do' stat 'using' S ',' runs 'in' cont" :=
+Notation "'do%return' a ':=' e 'whileb' expr 'do' stat 'using' runs 'in' cont" :=
   (do%return a := e
-   while result_success S (decide expr)
+   while result_success (decide expr)
    do stat
-   using S, runs
+   using runs
    in cont)
   (at level 50, left associativity) : monad_scope.
 
-Notation "'do%return' 'whileb' expr 'do' stat 'using' S ',' runs 'in' cont" :=
+Notation "'do%return' 'whileb' expr 'do' stat 'using' runs 'in' cont" :=
   (do%return
-   while result_success S (decide expr)
+   while result_success (decide expr)
    do stat
-   using S, runs
+   using runs
    in cont)
   (at level 50, left associativity) : monad_scope.
 
-Notation "'do%return' '(' a1 ',' a2 ')' ':=' e 'whileb' expr 'do' stat 'using' S ',' runs 'in' cont" :=
+Notation "'do%return' '(' a1 ',' a2 ')' ':=' e 'whileb' expr 'do' stat 'using' runs 'in' cont" :=
   (do%return (a1, a2) := e
-   while result_success S (decide expr)
+   while result_success (decide expr)
    do stat
-   using S, runs
+   using runs
    in cont)
   (at level 50, left associativity) : monad_scope.
 
-Notation "'do%return' '(' a1 ',' a2 ',' a3 ')' ':=' e 'whileb' expr 'do' stat 'using' S ',' runs 'in' cont" :=
+Notation "'do%return' '(' a1 ',' a2 ',' a3 ')' ':=' e 'whileb' expr 'do' stat 'using' runs 'in' cont" :=
   (do%return (a1, a2, a3) := e
-   while result_success S (decide expr)
+   while result_success (decide expr)
    do stat
-   using S, runs
+   using runs
    in cont)
   (at level 50, left associativity) : monad_scope.
 
-Notation "'do%return' '(' a1 ',' a2 ',' a3 ',' a4 ')' ':=' e 'whileb' expr 'do' stat 'using' S ',' runs 'in' cont" :=
+Notation "'do%return' '(' a1 ',' a2 ',' a3 ',' a4 ')' ':=' e 'whileb' expr 'do' stat 'using' runs 'in' cont" :=
   (do%return (a1, a2, a3, a4) := e
-   while result_success S (decide expr)
+   while result_success (decide expr)
    do stat
-   using S, runs
+   using runs
    in cont)
   (at level 50, left associativity) : monad_scope.
 
-Notation "'do%return' '(' a1 ',' a2 ',' a3 ',' a4 ',' a5 ')' ':=' e 'whileb' expr 'do' stat 'using' S ',' runs 'in' cont" :=
+Notation "'do%return' '(' a1 ',' a2 ',' a3 ',' a4 ',' a5 ')' ':=' e 'whileb' expr 'do' stat 'using' runs 'in' cont" :=
   (do%return (a1, a2, a3, a4, a5) := e
-   while result_success S (decide expr)
+   while result_success (decide expr)
    do stat
-   using S, runs
+   using runs
    in cont)
   (at level 50, left associativity) : monad_scope.
 
-Notation "'do%return' '(' a1 ',' a2 ',' a3 ',' a4 ',' a5 ',' a6 ')' ':=' e 'whileb' expr 'do' stat 'using' S ',' runs 'in' cont" :=
+Notation "'do%return' '(' a1 ',' a2 ',' a3 ',' a4 ',' a5 ',' a6 ')' ':=' e 'whileb' expr 'do' stat 'using' runs 'in' cont" :=
   (do%return (a1, a2, a3, a4, a5, a6) := e
-   while result_success S (decide expr)
+   while result_success (decide expr)
    do stat
-   using S, runs
+   using runs
    in cont)
   (at level 50, left associativity) : monad_scope.
 
 
-Notation "'fold%return' a ':=' e 'along' le 'as' l ',' l_ ',' l_list 'do' iterate 'using' S ',' runs ',' globals 'in' cont" :=
+Notation "'fold%return' a ':=' e 'along' le 'as' l ',' l_ ',' l_list 'do' iterate 'using' runs ',' globals 'in' cont" :=
   (let%exit a :=
      fold%let a := normal_result e
      along le
      as l, l_, l_list
-     do get_success S a (fun S a => iterate)
-     using S, runs, globals
-   using S in cont)
+     do get_success a (fun a => iterate)
+     using runs, globals
+    in cont)
   (at level 50, left associativity) : monad_scope.
 
-Notation "'fold%return' 'along' le 'as' l ',' l_ ',' l_list 'do' iterate 'using' S ',' runs ',' globals 'in' cont" :=
+Notation "'fold%return' 'along' le 'as' l ',' l_ ',' l_list 'do' iterate 'using' runs ',' globals 'in' cont" :=
   (fold%return ret := tt
    along le
    as l, l_, l_list
    do iterate
-   using S, runs, globals in
+   using runs, globals in
    cont)
   (at level 50, left associativity) : monad_scope.
 
-Notation "'fold%return' '(' a1 ',' a2 ')' ':=' e 'along' le 'as' l ',' l_ ',' l_list 'do' iterate 'using' S ',' runs ',' globals 'in' cont" :=
+Notation "'fold%return' '(' a1 ',' a2 ')' ':=' e 'along' le 'as' l ',' l_ ',' l_list 'do' iterate 'using' runs ',' globals 'in' cont" :=
   (fold%return a := e
    along le
    as l, l_, l_list
    do let (a1, a2) := a in iterate
-   using S, runs, globals in
+   using runs, globals in
    let (a1, a2) := a in
    cont)
   (at level 50, left associativity) : monad_scope.
 
-Notation "'fold%return' '(' a1 ',' a2 ',' a3 ')' ':=' e 'along' le 'as' l ',' l_ ',' l_list 'do' iterate 'using' S ',' runs ',' globals 'in' cont" :=
+Notation "'fold%return' '(' a1 ',' a2 ',' a3 ')' ':=' e 'along' le 'as' l ',' l_ ',' l_list 'do' iterate 'using' runs ',' globals 'in' cont" :=
   (fold%return a := e
    along le
    as l, l_, l_list
    do let (a1, a2, a3) := a in iterate
-   using S, runs, globals in
+   using runs, globals in
    let (a1, a2, a3) := a in
    cont)
   (at level 50, left associativity) : monad_scope.
 
-Notation "'fold%return' '(' a1 ',' a2 ',' a3 ',' a4 ')' ':=' e 'along' le 'as' l ',' l_ ',' l_list 'do' iterate 'using' S ',' runs ',' globals 'in' cont" :=
+Notation "'fold%return' '(' a1 ',' a2 ',' a3 ',' a4 ')' ':=' e 'along' le 'as' l ',' l_ ',' l_list 'do' iterate 'using' runs ',' globals 'in' cont" :=
   (fold%return a := e
    along le
    as l, l_, l_list
    do let (a1, a2, a3, a4) := a in iterate
-   using S, runs, globals in
+   using runs, globals in
    let (a1, a2, a3, a4) := a in
    cont)
   (at level 50, left associativity) : monad_scope.
 
-Notation "'fold%return' '(' a1 ',' a2 ',' a3 ',' a4 ',' a5 ')' ':=' e 'along' le 'as' l ',' l_ ',' l_list 'do' iterate 'using' S ',' runs ',' globals 'in' cont" :=
+Notation "'fold%return' '(' a1 ',' a2 ',' a3 ',' a4 ',' a5 ')' ':=' e 'along' le 'as' l ',' l_ ',' l_list 'do' iterate 'using' runs ',' globals 'in' cont" :=
   (fold%return a := e
    along le
    as l, l_, l_list
    do let (a1, a2, a3, a4, a5) := a in iterate
-   using S, runs, globals in
+   using runs, globals in
    let (a1, a2, a3, a4, a5) := a in
    cont)
   (at level 50, left associativity) : monad_scope.
 
-Notation "'fold%return' '(' a1 ',' a2 ',' a3 ',' a4 ',' a5 ',' a6 ')' ':=' e 'along' le 'as' l ',' l_ ',' l_list 'do' iterate 'using' S ',' runs ',' globals 'in' cont" :=
+Notation "'fold%return' '(' a1 ',' a2 ',' a3 ',' a4 ',' a5 ',' a6 ')' ':=' e 'along' le 'as' l ',' l_ ',' l_list 'do' iterate 'using' runs ',' globals 'in' cont" :=
   (fold%return a := e
    along le
    as l, l_, l_list
    do let (a1, a2, a3, a4, a5, a6) := a in iterate
-   using S, runs, globals in
+   using runs, globals in
    let (a1, a2, a3, a4, a5, a6) := a in
    cont)
   (at level 50, left associativity) : monad_scope.
 
 
-Notation "'fold%return' a ':=' e 'along' le 'as' l_car ',' l_tag 'do' iterate 'using' S ',' runs ',' globals 'in' cont" :=
+Notation "'fold%return' a ':=' e 'along' le 'as' l_car ',' l_tag 'do' iterate 'using' runs ',' globals 'in' cont" :=
   (let%exit a :=
      fold%let a := normal_result e
      along le
      as l_car, l_tag
-     do get_success S a (fun S a => iterate)
-     using S, runs, globals
-   using S in cont)
+     do get_success a (fun a => iterate)
+     using runs, globals
+    in cont)
   (at level 50, left associativity) : monad_scope.
 
-Notation "'fold%return' 'along' le 'as' l_car ',' l_tag 'do' iterate 'using' S ',' runs ',' globals 'in' cont" :=
+Notation "'fold%return' 'along' le 'as' l_car ',' l_tag 'do' iterate 'using' runs ',' globals 'in' cont" :=
   (fold%return ret := tt
    along le
    as l_car, l_tag
    do iterate
-   using S, runs, globals in
+   using runs, globals in
    cont)
   (at level 50, left associativity) : monad_scope.
 
-Notation "'fold%return' '(' a1 ',' a2 ')' ':=' e 'along' le 'as' l_car ',' l_tag 'do' iterate 'using' S ',' runs ',' globals 'in' cont" :=
+Notation "'fold%return' '(' a1 ',' a2 ')' ':=' e 'along' le 'as' l_car ',' l_tag 'do' iterate 'using' runs ',' globals 'in' cont" :=
   (fold%return a := e
    along le
    as l_car, l_tag
    do let (a1, a2) := a in iterate
-   using S, runs, globals in
+   using runs, globals in
    let (a1, a2) := a in
    cont)
   (at level 50, left associativity) : monad_scope.
 
-Notation "'fold%return' '(' a1 ',' a2 ',' a3 ')' ':=' e 'along' le 'as' l_car ',' l_tag 'do' iterate 'using' S ',' runs ',' globals 'in' cont" :=
+Notation "'fold%return' '(' a1 ',' a2 ',' a3 ')' ':=' e 'along' le 'as' l_car ',' l_tag 'do' iterate 'using' runs ',' globals 'in' cont" :=
   (fold%return a := e
    along le
    as l_car, l_tag
    do let (a1, a2, a3) := a in iterate
-   using S, runs, globals in
+   using runs, globals in
    let (a1, a2, a3) := a in
    cont)
   (at level 50, left associativity) : monad_scope.
 
-Notation "'fold%return' '(' a1 ',' a2 ',' a3 ',' a4 ')' ':=' e 'along' le 'as' l_car ',' l_tag 'do' iterate 'using' S ',' runs ',' globals 'in' cont" :=
+Notation "'fold%return' '(' a1 ',' a2 ',' a3 ',' a4 ')' ':=' e 'along' le 'as' l_car ',' l_tag 'do' iterate 'using' runs ',' globals 'in' cont" :=
   (fold%return a := e
    along le
    as l_car, l_tag
    do let (a1, a2, a3, a4) := a in iterate
-   using S, runs, globals in
+   using runs, globals in
    let (a1, a2, a3, a4) := a in
    cont)
   (at level 50, left associativity) : monad_scope.
 
-Notation "'fold%return' '(' a1 ',' a2 ',' a3 ',' a4 ',' a5 ')' ':=' e 'along' le 'as' l_car ',' l_tag 'do' iterate 'using' S ',' runs ',' globals 'in' cont" :=
+Notation "'fold%return' '(' a1 ',' a2 ',' a3 ',' a4 ',' a5 ')' ':=' e 'along' le 'as' l_car ',' l_tag 'do' iterate 'using' runs ',' globals 'in' cont" :=
   (fold%return a := e
    along le
    as l_car, l_tag
    do let (a1, a2, a3, a4, a5) := a in iterate
-   using S, runs, globals in
+   using runs, globals in
    let (a1, a2, a3, a4, a5) := a in
    cont)
   (at level 50, left associativity) : monad_scope.
 
-Notation "'fold%return' '(' a1 ',' a2 ',' a3 ',' a4 ',' a5 ',' a6 ')' ':=' e 'along' le 'as' l_car ',' l_tag 'do' iterate 'using' S ',' runs ',' globals 'in' cont" :=
+Notation "'fold%return' '(' a1 ',' a2 ',' a3 ',' a4 ',' a5 ',' a6 ')' ':=' e 'along' le 'as' l_car ',' l_tag 'do' iterate 'using' runs ',' globals 'in' cont" :=
   (fold%return a := e
    along le
    as l_car, l_tag
    do let (a1, a2, a3, a4, a5, a6) := a in iterate
-   using S, runs, globals in
+   using runs, globals in
    let (a1, a2, a3, a4, a5, a6) := a in
    cont)
   (at level 50, left associativity) : monad_scope.
 
-Notation "'fold%break' 'along' le 'as' l_car ',' l_tag 'do' iterate 'using' S ',' runs ',' globals 'in' cont" :=
+Notation "'fold%break' 'along' le 'as' l_car ',' l_tag 'do' iterate 'using' runs ',' globals 'in' cont" :=
   (run%success
      fold%return
      along le
      as l_car, l_tag
      do iterate
-     using S, runs, globals
-     in result_skip S
-   using S in cont)
+     using runs, globals
+     in result_skip
+    in cont)
   (at level 50, left associativity) : monad_scope.
 
-Notation "'fold%break' a ':=' e 'along' le 'as' l_car ',' l_tag 'do' iterate 'using' S ',' runs ',' globals 'in' cont" :=
+Notation "'fold%break' a ':=' e 'along' le 'as' l_car ',' l_tag 'do' iterate 'using' runs ',' globals 'in' cont" :=
   (let%success a :=
      fold%return a := e
      along le
      as l_car, l_tag
      do iterate
-     using S, runs, globals
-     in result_success S a
-   using S in cont)
+     using runs, globals
+     in result_success a
+    in cont)
     (at level 50, left associativity) : monad_scope.
 
-Notation "'fold%break' '(' a1 ',' a2 ')' ':=' e 'along' le 'as' l_car ',' l_tag 'do' iterate 'using' S ',' runs ',' globals 'in' cont" :=
+Notation "'fold%break' '(' a1 ',' a2 ')' ':=' e 'along' le 'as' l_car ',' l_tag 'do' iterate 'using' runs ',' globals 'in' cont" :=
   (let%success (a1, a2) :=
      fold%return (a1, a2) := e
      along le
      as l_car, l_tag
      do iterate
-     using S, runs, globals
-     in result_success S (a1, a2)
-   using S in cont)
+     using runs, globals
+     in result_success (a1, a2)
+    in cont)
   (at level 50, left associativity) : monad_scope.
 
-Notation "'fold%break' '(' a1 ',' a2 ',' a3 ')' ':=' e 'along' le 'as' l_car ',' l_tag 'do' iterate 'using' S ',' runs ',' globals 'in' cont" :=
+Notation "'fold%break' '(' a1 ',' a2 ',' a3 ')' ':=' e 'along' le 'as' l_car ',' l_tag 'do' iterate 'using' runs ',' globals 'in' cont" :=
   (let%success (a1, a2, a3) :=
      fold%return (a1, a2, a3) := e
      along le
      as l_car, l_tag
      do iterate
-     using S, runs, globals
-     in result_success S (a1, a2, a3)
-   using S in cont)
+     using runs, globals
+     in result_success (a1, a2, a3)
+    in cont)
   (at level 50, left associativity) : monad_scope.
 
-Notation "'fold%break' '(' a1 ',' a2 ',' a3 ',' a4 ')' ':=' e 'along' le 'as' l_car ',' l_tag 'do' iterate 'using' S ',' runs ',' globals 'in' cont" :=
+Notation "'fold%break' '(' a1 ',' a2 ',' a3 ',' a4 ')' ':=' e 'along' le 'as' l_car ',' l_tag 'do' iterate 'using' runs ',' globals 'in' cont" :=
   (let%success (a1, a2, a3, a4) :=
      fold%return (a1, a2, a3, a4) := e
      along le
      as l_car, l_tag
      do iterate
-     using S, runs, globals
-     in result_success S (a1, a2, a3, a4)
-   using S in cont)
+     using runs, globals
+     in result_success (a1, a2, a3, a4)
+    in cont)
   (at level 50, left associativity) : monad_scope.
 
-Notation "'fold%break' '(' a1 ',' a2 ',' a3 ',' a4 ',' a5 ')' ':=' e 'along' le 'as' l_car ',' l_tag 'do' iterate 'using' S ',' runs ',' globals 'in' cont" :=
+Notation "'fold%break' '(' a1 ',' a2 ',' a3 ',' a4 ',' a5 ')' ':=' e 'along' le 'as' l_car ',' l_tag 'do' iterate 'using' runs ',' globals 'in' cont" :=
   (let%success (a1, a2, a3, a4, a5) :=
      fold%return (a1, a2, a3, a4, a5) := e
      along le
      as l_car, l_tag
      do iterate
-     using S, runs, globals
-     in result_success S (a1, a2, a3, a4, a5)
-   using S in cont)
+     using runs, globals
+     in result_success (a1, a2, a3, a4, a5)
+    in cont)
   (at level 50, left associativity) : monad_scope.
 
 
@@ -1020,21 +1020,22 @@ Notation "'fold%break' '(' a1 ',' a2 ',' a3 ',' a4 ',' a5 ')' ':=' e 'along' le 
   as it was when calling [setjmp] the first time, but with the value returned by the
   [result_longjump] costructor instead of the default one. **)
 
-Definition set_longjump runs (A : Type) S mask (cjmpbuf : nat) (f : state -> context_type -> result A) : result A :=
-  match f S mask with
-  | result_success S0 a => result_success S0 a
-  | result_longjump S0 n mask =>
-    ifb cjmpbuf = n then
-      runs_set_longjump runs S0 mask cjmpbuf f
-    else result_longjump S0 n mask
-  | result_error_stack S0 stack s => result_error_stack S0 stack s
-  | result_impossible_stack S0 stack s => result_impossible_stack S0 stack s
-  | result_not_implemented_stack stack s => result_not_implemented_stack stack s
-  | result_bottom S0 => result_bottom S0
-  end.
+Definition set_longjump runs (A : Type) mask (cjmpbuf : nat) (f : context_type -> result A) : result A :=
+  fun S =>
+    match f mask S with
+    | result_success a S0 => result_success a S0
+    | result_longjump n mask S0 =>
+      ifb cjmpbuf = n then
+        runs_set_longjump runs mask cjmpbuf f S0
+      else result_longjump n mask S0
+    | result_error_stack stack s S0 => result_error_stack stack s S0
+    | result_impossible_stack stack s S0 => result_impossible_stack stack s S0
+    | result_not_implemented_stack stack s => result_not_implemented_stack stack s
+    | result_bottom S0 => result_bottom S0
+    end.
 
-Notation "'set%longjump' cjmpbuf 'as' ret 'using' S ',' runs 'in' cont" :=
-  (set_longjump runs S empty_context_type cjmpbuf (fun S ret => cont))
+Notation "'set%longjump' cjmpbuf 'as' ret 'using' runs 'in' cont" :=
+  (set_longjump runs empty_context_type cjmpbuf (fun S ret => cont))
   (at level 50, left associativity) : monad_scope.
 
 
@@ -1044,419 +1045,397 @@ Notation "'set%longjump' cjmpbuf 'as' ret 'using' S ',' runs 'in' cont" :=
 
 (** ** Along Lists **)
 
-Definition for_list A B S (a : A) (l : list B) body :=
+Definition for_list A B (a : A) (l : list B) body :=
   fold_left (fun i (r : result A) =>
-      let%success a := r using S in
-      body S a i)
-    (result_success S a) l.
+      let%success a := r  in
+      body a i)
+    (result_success a) l.
 
-Notation "'do%let' a ':=' e 'for' i 'in%list' l 'do' body 'using' S" :=
-  (for_list S e l (fun S a i => body))
+Notation "'do%let' a ':=' e 'for' i 'in%list' l 'do' body" :=
+  (for_list e l (fun a i => body))
   (at level 50, left associativity) : monad_scope.
 
-Notation "'do%let' 'for' i 'in%list' l 'do' body 'using' S" :=
-  (do%let _ := tt for i in%list l do body using S)
+Notation "'do%let' 'for' i 'in%list' l 'do' body" :=
+  (do%let _ := tt for i in%list l do body)
   (at level 50, left associativity) : monad_scope.
 
-Notation "'do%let' '(' a1 ',' a2 ')' ':=' a 'for' i 'in%list' l 'do' body 'using' S" :=
+Notation "'do%let' '(' a1 ',' a2 ')' ':=' a 'for' i 'in%list' l 'do' body" :=
   (do%let x := a for i in%list l
-   do let (a1, a2) := x in body using S)
+   do let (a1, a2) := x in body)
   (at level 50, left associativity) : monad_scope.
 
-Notation "'do%let' '(' a1 ',' a2 ',' a3 ')' ':=' a 'for' i 'in%list' l 'do' body 'using' S" :=
+Notation "'do%let' '(' a1 ',' a2 ',' a3 ')' ':=' a 'for' i 'in%list' l 'do' body" :=
   (do%let x := a for i in%list l
-   do let '(a1, a2, a3) := x in body using S)
+   do let '(a1, a2, a3) := x in body)
   (at level 50, left associativity) : monad_scope.
 
-Notation "'do%let' '(' a1 ',' a2 ',' a3 ',' a4 ')' ':=' a 'for' i 'in%list' l 'do' body 'using' S" :=
+Notation "'do%let' '(' a1 ',' a2 ',' a3 ',' a4 ')' ':=' a 'for' i 'in%list' l 'do' body" :=
   (do%let x := a for i in%list l
-   do let '(a1, a2, a3, a4) := x in body using S)
+   do let '(a1, a2, a3, a4) := x in body)
   (at level 50, left associativity) : monad_scope.
 
-Notation "'do%let' '(' a1 ',' a2 ',' a3 ',' a4 ',' a5 ')' ':=' a 'for' i 'in%list' l 'do' body 'using' S" :=
+Notation "'do%let' '(' a1 ',' a2 ',' a3 ',' a4 ',' a5 ')' ':=' a 'for' i 'in%list' l 'do' body" :=
   (do%let x := a for i in%list l
-   do let '(a1, a2, a3, a4, a5) := x in body using S)
+   do let '(a1, a2, a3, a4, a5) := x in body)
   (at level 50, left associativity) : monad_scope.
 
-Notation "'do%let' '(' a1 ',' a2 ',' a3 ',' a4 ',' a5 ',' a6 ')' ':=' a 'for' i 'in%list' l 'do' body 'using' S" :=
+Notation "'do%let' '(' a1 ',' a2 ',' a3 ',' a4 ',' a5 ',' a6 ')' ':=' a 'for' i 'in%list' l 'do' body" :=
   (do%let x := a for i in%list l
-   do let '(a1, a2, a3, a4, a5, a6) := x in body using S)
+   do let '(a1, a2, a3, a4, a5, a6) := x in body)
   (at level 50, left associativity) : monad_scope.
 
-Notation "'do%success' 'for' i 'in%list' l 'do' body 'using' S 'in' cont" :=
+Notation "'do%success' 'for' i 'in%list' l 'do' body 'in' cont" :=
   (run%success
      do%let for i in%list l
-     do body
-     using S using S in
+     do body in
    cont)
   (at level 50, left associativity) : monad_scope.
 
-Notation "'do%success' a ':=' e 'for' i 'in%list' l 'do' body 'using' S 'in' cont" :=
+Notation "'do%success' a ':=' e 'for' i 'in%list' l 'do' body 'in' cont" :=
   (let%success a :=
      do%let a := e
      for i in%list l
-     do body
-     using S using S in
+     do body in
    cont)
   (at level 50, left associativity) : monad_scope.
 
-Notation "'do%success' '(' a1 ',' a2 ')' ':=' e 'for' i 'in%list' l 'do' body 'using' S 'in' cont" :=
+Notation "'do%success' '(' a1 ',' a2 ')' ':=' e 'for' i 'in%list' l 'do' body 'in' cont" :=
   (let%success (a1, a2) :=
      do%let (a1, a2) := e
      for i in%list l
-     do body
-     using S using S in
+     do body in
    cont)
   (at level 50, left associativity) : monad_scope.
 
-Notation "'do%success' '(' a1 ',' a2 ',' a3 ')' ':=' e 'for' i 'in%list' l 'do' body 'using' S 'in' cont" :=
+Notation "'do%success' '(' a1 ',' a2 ',' a3 ')' ':=' e 'for' i 'in%list' l 'do' body 'in' cont" :=
   (let%success (a1, a2, a3) :=
      do%let (a1, a2, a3) := e
      for i in%list l
-     do body
-     using S using S in
+     do body in
    cont)
   (at level 50, left associativity) : monad_scope.
 
-Notation "'do%success' '(' a1 ',' a2 ',' a3 ',' a4 ')' ':=' e 'for' i 'in%list' l 'do' body 'using' S 'in' cont" :=
+Notation "'do%success' '(' a1 ',' a2 ',' a3 ',' a4 ')' ':=' e 'for' i 'in%list' l 'do' body 'in' cont" :=
   (let%success (a1, a2, a3, a4) :=
      do%let (a1, a2, a3, a4) := e
      for i in%list l
-     do body
-     using S using S in
+     do body in
    cont)
   (at level 50, left associativity) : monad_scope.
 
-Notation "'do%success' '(' a1 ',' a2 ',' a3 ',' a4 ',' a5 ')' ':=' e 'for' i 'in%list' l 'do' body 'using' S 'in' cont" :=
+Notation "'do%success' '(' a1 ',' a2 ',' a3 ',' a4 ',' a5 ')' ':=' e 'for' i 'in%list' l 'do' body 'in' cont" :=
   (let%success (a1, a2, a3, a4, a5) :=
      do%let (a1, a2, a3, a4, a5) := e
      for i in%list l
-     do body
-     using S using S in
+     do body in
    cont)
   (at level 50, left associativity) : monad_scope.
 
-Notation "'do%success' '(' a1 ',' a2 ',' a3 ',' a4 ',' a5 ',' a6 ')' ':=' e 'for' i 'in%list' l 'do' body 'using' S 'in' cont" :=
+Notation "'do%success' '(' a1 ',' a2 ',' a3 ',' a4 ',' a5 ',' a6 ')' ':=' e 'for' i 'in%list' l 'do' body 'in' cont" :=
   (let%success (a1, a2, a3, a4, a5, a6) :=
      do%let (a1, a2, a3, a4, a5, a6) := e
      for i in%list l
-     do body
-     using S using S in
+     do body in
    cont)
   (at level 50, left associativity) : monad_scope.
 
 
 (** ** Along Intervals **)
 
-Definition for_loop A S (a : A) (start : nat) (last : int) body :=
+Definition for_loop A (a : A) (start : nat) (last : int) body :=
   ifb last < start then
-    result_success S a
+    result_success a
   else
     (** We know that [last >= 0]. **)
     do%let x := a
     for i in%list seq start (1 + Z.to_nat last - start) do
-      body S x i using S.
+      body x i.
 
-Notation "'do%let' a ':=' e 'for' i 'from' start 'to' last 'do' body 'using' S" :=
-  (for_loop S e start last (fun S a i => body))
+Notation "'do%let' a ':=' e 'for' i 'from' start 'to' last 'do' body" :=
+  (for_loop e start last (fun a i => body))
   (at level 50, left associativity) : monad_scope.
 
-Notation "'do%let' 'for' i 'from' start 'to' last 'do' body 'using' S" :=
-  (do%let _ := tt for i from start to last do body using S)
+Notation "'do%let' 'for' i 'from' start 'to' last 'do' body" :=
+  (do%let _ := tt for i from start to last do body)
   (at level 50, left associativity) : monad_scope.
 
-Notation "'do%let' '(' a1 ',' a2 ')' ':=' a 'for' i 'from' start 'to' last 'do' body 'using' S" :=
+Notation "'do%let' '(' a1 ',' a2 ')' ':=' a 'for' i 'from' start 'to' last 'do' body" :=
   (do%let x := a for i from start to last
-   do let (a1, a2) := x in body using S)
+   do let (a1, a2) := x in body)
   (at level 50, left associativity) : monad_scope.
 
-Notation "'do%let' '(' a1 ',' a2 ',' a3 ')' ':=' a 'for' i 'from' start 'to' last 'do' body 'using' S" :=
+Notation "'do%let' '(' a1 ',' a2 ',' a3 ')' ':=' a 'for' i 'from' start 'to' last 'do' body" :=
   (do%let x := a for i from start to last
-   do let '(a1, a2, a3) := x in body using S)
+   do let '(a1, a2, a3) := x in body)
   (at level 50, left associativity) : monad_scope.
 
-Notation "'do%let' '(' a1 ',' a2 ',' a3 ',' a4 ')' ':=' a 'for' i 'from' start 'to' last 'do' body 'using' S" :=
+Notation "'do%let' '(' a1 ',' a2 ',' a3 ',' a4 ')' ':=' a 'for' i 'from' start 'to' last 'do' body" :=
   (do%let x := a for i from start to last
-   do let '(a1, a2, a3, a4) := x in body using S)
+   do let '(a1, a2, a3, a4) := x in body)
   (at level 50, left associativity) : monad_scope.
 
-Notation "'do%let' '(' a1 ',' a2 ',' a3 ',' a4 ',' a5 ')' ':=' a 'for' i 'from' start 'to' last 'do' body 'using' S" :=
+Notation "'do%let' '(' a1 ',' a2 ',' a3 ',' a4 ',' a5 ')' ':=' a 'for' i 'from' start 'to' last 'do' body" :=
   (do%let x := a for i from start to last
-   do let '(a1, a2, a3, a4, a5) := x in body using S)
+   do let '(a1, a2, a3, a4, a5) := x in body)
   (at level 50, left associativity) : monad_scope.
 
-Notation "'do%let' '(' a1 ',' a2 ',' a3 ',' a4 ',' a5 ',' a6 ')' ':=' a 'for' i 'from' start 'to' last 'do' body 'using' S" :=
+Notation "'do%let' '(' a1 ',' a2 ',' a3 ',' a4 ',' a5 ',' a6 ')' ':=' a 'for' i 'from' start 'to' last 'do' body" :=
   (do%let x := a for i from start to last
-   do let '(a1, a2, a3, a4, a5, a6) := x in body using S)
+   do let '(a1, a2, a3, a4, a5, a6) := x in body)
   (at level 50, left associativity) : monad_scope.
 
-Notation "'do%success' 'for' i 'from' start 'to' last 'do' body 'using' S 'in' cont" :=
+Notation "'do%success' 'for' i 'from' start 'to' last 'do' body 'in' cont" :=
   (run%success
      do%let for i from start to last
-     do body
-     using S using S in
+     do body in
    cont)
   (at level 50, left associativity) : monad_scope.
 
-Notation "'do%success' a ':=' e 'for' i 'from' start 'to' last 'do' body 'using' S 'in' cont" :=
+Notation "'do%success' a ':=' e 'for' i 'from' start 'to' last 'do' body 'in' cont" :=
   (let%success a :=
      do%let a := e
      for i from start to last
-     do body
-     using S using S in
+     do body in
    cont)
   (at level 50, left associativity) : monad_scope.
 
-Notation "'do%success' '(' a1 ',' a2 ')' ':=' e 'for' i 'from' start 'to' last 'do' body 'using' S 'in' cont" :=
+Notation "'do%success' '(' a1 ',' a2 ')' ':=' e 'for' i 'from' start 'to' last 'do' body 'in' cont" :=
   (let%success (a1, a2) :=
      do%let (a1, a2) := e
      for i from start to last
-     do body
-     using S using S in
+     do body in
    cont)
   (at level 50, left associativity) : monad_scope.
 
-Notation "'do%success' '(' a1 ',' a2 ',' a3 ')' ':=' e 'for' i 'from' start 'to' last 'do' body 'using' S 'in' cont" :=
+Notation "'do%success' '(' a1 ',' a2 ',' a3 ')' ':=' e 'for' i 'from' start 'to' last 'do' body 'in' cont" :=
   (let%success (a1, a2, a3) :=
      do%let (a1, a2, a3) := e
      for i from start to last
-     do body
-     using S using S in
+     do body in
    cont)
   (at level 50, left associativity) : monad_scope.
 
-Notation "'do%success' '(' a1 ',' a2 ',' a3 ',' a4 ')' ':=' e 'for' i 'from' start 'to' last 'do' body 'using' S 'in' cont" :=
+Notation "'do%success' '(' a1 ',' a2 ',' a3 ',' a4 ')' ':=' e 'for' i 'from' start 'to' last 'do' body 'in' cont" :=
   (let%success (a1, a2, a3, a4) :=
      do%let (a1, a2, a3, a4) := e
      for i from start to last
-     do body
-     using S using S in
+     do body in
    cont)
   (at level 50, left associativity) : monad_scope.
 
-Notation "'do%success' '(' a1 ',' a2 ',' a3 ',' a4 ',' a5 ')' ':=' e 'for' i 'from' start 'to' last 'do' body 'using' S 'in' cont" :=
+Notation "'do%success' '(' a1 ',' a2 ',' a3 ',' a4 ',' a5 ')' ':=' e 'for' i 'from' start 'to' last 'do' body 'in' cont" :=
   (let%success (a1, a2, a3, a4, a5) :=
      do%let (a1, a2, a3, a4, a5) := e
      for i from start to last
-     do body
-     using S using S in
+     do body in
    cont)
   (at level 50, left associativity) : monad_scope.
 
-Notation "'do%success' '(' a1 ',' a2 ',' a3 ',' a4 ',' a5 ',' a6 ')' ':=' e 'for' i 'from' start 'to' last 'do' body 'using' S 'in' cont" :=
+Notation "'do%success' '(' a1 ',' a2 ',' a3 ',' a4 ',' a5 ',' a6 ')' ':=' e 'for' i 'from' start 'to' last 'do' body 'in' cont" :=
   (let%success (a1, a2, a3, a4, a5, a6) :=
      do%let (a1, a2, a3, a4, a5, a6) := e
      for i from start to last
-     do body
-     using S using S in
+     do body in
    cont)
   (at level 50, left associativity) : monad_scope.
 
-Notation "'do%exit' a ':=' e 'for' i 'from' start 'to' last 'do' body 'using' S 'in' cont" :=
+Notation "'do%exit' a ':=' e 'for' i 'from' start 'to' last 'do' body 'in' cont" :=
   (let%exit a :=
      do%let ret := normal_result e
      for i from start to last
-     do get_success S ret (fun S a => body)
-     using S using S in
+     do get_success ret (fun a => body) in
    cont)
   (at level 50, left associativity) : monad_scope.
 
-Notation "'do%exit' 'for' i 'from' start 'to' last 'do' body 'using' S 'in' cont" :=
+Notation "'do%exit' 'for' i 'from' start 'to' last 'do' body 'in' cont" :=
   (do%exit _ := tt
    for i from start to last
-   do body using S
-   in cont)
+   do body in
+   cont)
   (at level 50, left associativity) : monad_scope.
 
-Notation "'do%exit' '(' a1 ',' a2 ')' ':=' e 'for' i 'from' start 'to' last 'do' body 'using' S 'in' cont" :=
+Notation "'do%exit' '(' a1 ',' a2 ')' ':=' e 'for' i 'from' start 'to' last 'do' body 'in' cont" :=
   (do%exit a := e
    for i from start to last
-   do let (a1, a2) := a in body using S
+   do let (a1, a2) := a in body
    in let (a1, a2) := a in cont)
   (at level 50, left associativity) : monad_scope.
 
-Notation "'do%exit' '(' a1 ',' a2 ',' a3 ')' ':=' e 'for' i 'from' start 'to' last 'do' body 'using' S 'in' cont" :=
+Notation "'do%exit' '(' a1 ',' a2 ',' a3 ')' ':=' e 'for' i 'from' start 'to' last 'do' body 'in' cont" :=
   (do%exit a := e
    for i from start to last
-   do let '(a1, a2, a3) := a in body using S
+   do let '(a1, a2, a3) := a in body
    in let '(a1, a2, a3) := a in cont)
   (at level 50, left associativity) : monad_scope.
 
-Notation "'do%exit' '(' a1 ',' a2 ',' a3 ',' a4 ')' ':=' e 'for' i 'from' start 'to' last 'do' body 'using' S 'in' cont" :=
+Notation "'do%exit' '(' a1 ',' a2 ',' a3 ',' a4 ')' ':=' e 'for' i 'from' start 'to' last 'do' body 'in' cont" :=
   (do%exit a := e
    for i from start to last
-   do let '(a1, a2, a3, a4) := a in body using S
+   do let '(a1, a2, a3, a4) := a in body
    in let '(a1, a2, a3, a4) := a in cont)
   (at level 50, left associativity) : monad_scope.
 
-Notation "'do%exit' '(' a1 ',' a2 ',' a3 ',' a4 ',' a5 ')' ':=' e 'for' i 'from' start 'to' last 'do' body 'using' S 'in' cont" :=
+Notation "'do%exit' '(' a1 ',' a2 ',' a3 ',' a4 ',' a5 ')' ':=' e 'for' i 'from' start 'to' last 'do' body 'in' cont" :=
   (do%exit a := e
    for i from start to last
-   do let '(a1, a2, a3, a4, a5) := a in body using S
+   do let '(a1, a2, a3, a4, a5) := a in body
    in let '(a1, a2, a3, a4, a5) := a in cont)
   (at level 50, left associativity) : monad_scope.
 
-Notation "'do%exit' '(' a1 ',' a2 ',' a3 ',' a4 ',' a5 ',' a6 ')' ':=' e 'for' i 'from' start 'to' last 'do' body 'using' S 'in' cont" :=
+Notation "'do%exit' '(' a1 ',' a2 ',' a3 ',' a4 ',' a5 ',' a6 ')' ':=' e 'for' i 'from' start 'to' last 'do' body 'in' cont" :=
   (do%exit a := e
    for i from start to last
-   do let '(a1, a2, a3, a4, a5, a6) := a in body using S
+   do let '(a1, a2, a3, a4, a5, a6) := a in body
    in let '(a1, a2, a3, a4, a5, a6) := a in cont)
   (at level 50, left associativity) : monad_scope.
 
-Notation "'do%break' 'for' i 'from' start 'to' last 'do' body 'using' S 'in' cont" :=
+Notation "'do%break' 'for' i 'from' start 'to' last 'do' body 'in' cont" :=
   (run%success
      do%exit
      for i from start to last
-     do body using S
-     in result_skip S using S
+     do body
+     in result_skip
    in cont)
   (at level 50, left associativity) : monad_scope.
 
-Notation "'do%break' a ':=' e 'for' i 'from' start 'to' last 'do' body 'using' S 'in' cont" :=
+Notation "'do%break' a ':=' e 'for' i 'from' start 'to' last 'do' body 'in' cont" :=
   (let%success a :=
      do%exit a := e
      for i from start to last
-     do body using S
-     in result_success S a using S
+     do body
+     in result_success a
    in cont)
   (at level 50, left associativity) : monad_scope.
 
-Notation "'do%break' '(' a1 ',' a2 ')' ':=' e 'for' i 'from' start 'to' last 'do' body 'using' S 'in' cont" :=
+Notation "'do%break' '(' a1 ',' a2 ')' ':=' e 'for' i 'from' start 'to' last 'do' body 'in' cont" :=
   (let%success (a1, a2) :=
      do%exit (a1, a2) := e
      for i from start to last
-     do body using S
-     in result_success S (a1, a2) using S
+     do body
+     in result_success (a1, a2)
    in cont)
   (at level 50, left associativity) : monad_scope.
 
-Notation "'do%break' '(' a1 ',' a2 ',' a3 ')' ':=' e 'for' i 'from' start 'to' last 'do' body 'using' S 'in' cont" :=
+Notation "'do%break' '(' a1 ',' a2 ',' a3 ')' ':=' e 'for' i 'from' start 'to' last 'do' body 'in' cont" :=
   (let%success (a1, a2, a3) :=
      do%exit (a1, a2, a3) := e
      for i from start to last
-     do body using S
-     in result_success S (a1, a2, a3) using S
+     do body
+     in result_success (a1, a2, a3)
    in cont)
   (at level 50, left associativity) : monad_scope.
 
-Notation "'do%break' '(' a1 ',' a2 ',' a3 ',' a4 ')' ':=' e 'for' i 'from' start 'to' last 'do' body 'using' S 'in' cont" :=
+Notation "'do%break' '(' a1 ',' a2 ',' a3 ',' a4 ')' ':=' e 'for' i 'from' start 'to' last 'do' body 'in' cont" :=
   (let%success (a1, a2, a3, a4) :=
      do%exit (a1, a2, a3, a4) := e
      for i from start to last
-     do body using S
-     in result_success S (a1, a2, a3, a4) using S
+     do body
+     in result_success (a1, a2, a3, a4)
    in cont)
   (at level 50, left associativity) : monad_scope.
 
-Notation "'do%break' '(' a1 ',' a2 ',' a3 ',' a4 ',' a5 ')' ':=' e 'for' i 'from' start 'to' last 'do' body 'using' S 'in' cont" :=
+Notation "'do%break' '(' a1 ',' a2 ',' a3 ',' a4 ',' a5 ')' ':=' e 'for' i 'from' start 'to' last 'do' body 'in' cont" :=
   (let%success (a1, a2, a3, a4, a5) :=
      do%exit (a1, a2, a3, a4, a5) := e
      for i from start to last
-     do body using S
-     in result_success S (a1, a2, a3, a4, a5) using S
+     do body
+     in result_success (a1, a2, a3, a4, a5)
    in cont)
   (at level 50, left associativity) : monad_scope.
 
 
 (** ** Along Arrays **)
 
-Definition for_array A B S (a : A) (array : ArrayList.array B) body :=
+Definition for_array A B (a : A) (array : ArrayList.array B) body :=
   do%let x := a
   for i in%list ArrayList.to_list array do
-    body S x i using S.
+    body x i.
 
-Notation "'do%let' a ':=' e 'for' i 'in%array' array 'do' body 'using' S" :=
-  (for_array S e array (fun S a i => body))
+Notation "'do%let' a ':=' e 'for' i 'in%array' array 'do' body" :=
+  (for_array e array (fun a i => body))
   (at level 50, left associativity) : monad_scope.
 
-Notation "'do%let' 'for' i 'in%array' array 'do' body 'using' S" :=
-  (do%let _ := tt for i in%array array do body using S)
+Notation "'do%let' 'for' i 'in%array' array 'do' body" :=
+  (do%let _ := tt for i in%array array do body)
   (at level 50, left associativity) : monad_scope.
 
-Notation "'do%let' '(' a1 ',' a2 ')' ':=' a 'for' i 'in%array' array 'do' body 'using' S" :=
+Notation "'do%let' '(' a1 ',' a2 ')' ':=' a 'for' i 'in%array' array 'do' body" :=
   (do%let x := a for i in%array array
-   do let (a1, a2) := x in body using S)
+   do let (a1, a2) := x in body)
   (at level 50, left associativity) : monad_scope.
 
-Notation "'do%let' '(' a1 ',' a2 ',' a3 ')' ':=' a 'for' i 'in%array' array 'do' body 'using' S" :=
+Notation "'do%let' '(' a1 ',' a2 ',' a3 ')' ':=' a 'for' i 'in%array' array 'do' body" :=
   (do%let x := a for i in%array array
-   do let '(a1, a2, a3) := x in body using S)
+   do let '(a1, a2, a3) := x in body)
   (at level 50, left associativity) : monad_scope.
 
-Notation "'do%let' '(' a1 ',' a2 ',' a3 ',' a4 ')' ':=' a 'for' i 'in%array' array 'do' body 'using' S" :=
+Notation "'do%let' '(' a1 ',' a2 ',' a3 ',' a4 ')' ':=' a 'for' i 'in%array' array 'do' body" :=
   (do%let x := a for i in%array array
-   do let '(a1, a2, a3, a4) := x in body using S)
+   do let '(a1, a2, a3, a4) := x in body)
   (at level 50, left associativity) : monad_scope.
 
-Notation "'do%let' '(' a1 ',' a2 ',' a3 ',' a4 ',' a5 ')' ':=' a 'for' i 'in%array' array 'do' body 'using' S" :=
+Notation "'do%let' '(' a1 ',' a2 ',' a3 ',' a4 ',' a5 ')' ':=' a 'for' i 'in%array' array 'do' body" :=
   (do%let x := a for i in%array array
-   do let '(a1, a2, a3, a4, a5) := x in body using S)
+   do let '(a1, a2, a3, a4, a5) := x in body)
   (at level 50, left associativity) : monad_scope.
 
-Notation "'do%let' '(' a1 ',' a2 ',' a3 ',' a4 ',' a5 ',' a6 ')' ':=' a 'for' i 'in%array' array 'do' body 'using' S" :=
+Notation "'do%let' '(' a1 ',' a2 ',' a3 ',' a4 ',' a5 ',' a6 ')' ':=' a 'for' i 'in%array' array 'do' body" :=
   (do%let x := a for i in%array array
-   do let '(a1, a2, a3, a4, a5, a6) := x in body using S)
+   do let '(a1, a2, a3, a4, a5, a6) := x in body)
   (at level 50, left associativity) : monad_scope.
 
-Notation "'do%success' 'for' i 'in%array' array 'do' body 'using' S 'in' cont" :=
+Notation "'do%success' 'for' i 'in%array' array 'do' body 'in' cont" :=
   (run%success
      do%let for i in%array array
-     do body
-     using S using S in
+     do body in
    cont)
   (at level 50, left associativity) : monad_scope.
 
-Notation "'do%success' a ':=' e 'for' i 'in%array' array 'do' body 'using' S 'in' cont" :=
+Notation "'do%success' a ':=' e 'for' i 'in%array' array 'do' body 'in' cont" :=
   (let%success a :=
      do%let a := e
      for i in%array array
-     do body
-     using S using S in
+     do body in
    cont)
   (at level 50, left associativity) : monad_scope.
 
-Notation "'do%success' '(' a1 ',' a2 ')' ':=' e 'for' i 'in%array' array 'do' body 'using' S 'in' cont" :=
+Notation "'do%success' '(' a1 ',' a2 ')' ':=' e 'for' i 'in%array' array 'do' body 'in' cont" :=
   (let%success (a1, a2) :=
      do%let (a1, a2) := e
      for i in%array array
-     do body
-     using S using S in
+     do body in
    cont)
   (at level 50, left associativity) : monad_scope.
 
-Notation "'do%success' '(' a1 ',' a2 ',' a3 ')' ':=' e 'for' i 'in%array' array 'do' body 'using' S 'in' cont" :=
+Notation "'do%success' '(' a1 ',' a2 ',' a3 ')' ':=' e 'for' i 'in%array' array 'do' body 'in' cont" :=
   (let%success (a1, a2, a3) :=
      do%let (a1, a2, a3) := e
      for i in%array array
-     do body
-     using S using S in
+     do body in
    cont)
   (at level 50, left associativity) : monad_scope.
 
-Notation "'do%success' '(' a1 ',' a2 ',' a3 ',' a4 ')' ':=' e 'for' i 'in%array' array 'do' body 'using' S 'in' cont" :=
+Notation "'do%success' '(' a1 ',' a2 ',' a3 ',' a4 ')' ':=' e 'for' i 'in%array' array 'do' body 'in' cont" :=
   (let%success (a1, a2, a3, a4) :=
      do%let (a1, a2, a3, a4) := e
      for i in%array array
-     do body
-     using S using S in
+     do body in
    cont)
   (at level 50, left associativity) : monad_scope.
 
-Notation "'do%success' '(' a1 ',' a2 ',' a3 ',' a4 ',' a5 ')' ':=' e 'for' i 'in%array' array 'do' body 'using' S 'in' cont" :=
+Notation "'do%success' '(' a1 ',' a2 ',' a3 ',' a4 ',' a5 ')' ':=' e 'for' i 'in%array' array 'do' body 'in' cont" :=
   (let%success (a1, a2, a3, a4, a5) :=
      do%let (a1, a2, a3, a4, a5) := e
      for i in%array array
-     do body
-     using S using S in
+     do body in
    cont)
   (at level 50, left associativity) : monad_scope.
 
-Notation "'do%success' '(' a1 ',' a2 ',' a3 ',' a4 ',' a5 ',' a6 ')' ':=' e 'for' i 'in%array' array 'do' body 'using' S 'in' cont" :=
+Notation "'do%success' '(' a1 ',' a2 ',' a3 ',' a4 ',' a5 ',' a6 ')' ':=' e 'for' i 'in%array' array 'do' body 'in' cont" :=
   (let%success (a1, a2, a3, a4, a5, a6) :=
      do%let (a1, a2, a3, a4, a5, a6) := e
      for i in%array array
-     do body
-     using S using S in
+     do body in
    cont)
   (at level 50, left associativity) : monad_scope.
 
